adapt the old proof

Protocols/RBABC/Protocol.v
@@ -1,11 +1,36 @@
 From Coq Require Import Bool List PeanoNat.
 From Coq Require ssrbool.
 Import (coercions) ssrbool.
-From ABCProtocol.Systems Require Export Protocol.
+From ABCProtocol.Composition Require Export Protocol.
 From ABCProtocol.Protocols.RBABC Require Export Types.
 From ABCProtocol.Protocols.ABC Require Import Protocol.
 From ABCProtocol.Protocols.RB Require Import Protocol.
 
+Module RBACTrigger (A : NetAddr) (R : Round) (ARP : AddrRoundPair A R) (Sn : Signable) (V : SignableValue Sn) (VBFT : ValueBFT A R V) 
+  (BTh : ClassicByzThreshold A) (RBM : RBMessage A R V)
+  (P : PKI A Sn) (TSS0 : ThresholdSignatureSchemePrim A Sn with Definition thres := BTh.t0) (* ! *)
+  (TSS : ThresholdSignatureScheme A Sn with Module TSSPrim := TSS0)
+  (ACDT : ACDataTypes A Sn V P TSS) 
+  (CC : CertCheckers A Sn V P TSS ACDT) (ACM : ACMessage A Sn V P TSS ACDT)
+  (M : CompMessage RBM ACM)
+  (RBPk : SimplePacket A RBM) (ACPk : SimplePacket A ACM) 
+  (RBP : RBProtocol A R V VBFT BTh RBM RBPk)
+  (ACP : ACProtocol A Sn V BTh P TSS0 TSS ACDT CC ACM ACPk) <: SeqCompProtocolTrigger A RBM ACM BTh RBPk ACPk RBP ACP.
+
+Import ARP.
+
+Definition trigger_procMsg (st st' : RBP.State) :=
+  match (st.(RBP.output) arp), (st'.(RBP.output) arp) with
+  | nil, nil => None
+  | _ :: _, _ => None
+  | nil, v :: _ => Some (ACP.SubmitIntTrans v)
+  end.
+
+Definition trigger_procInt : RBP.State -> RBP.State -> option ACP.InternalTransition := fun _ _ => None.
+
+End RBACTrigger.
+
+(*
 From RecordUpdate Require Import RecordUpdate.
 
 Module Type RBACProtocol (A : NetAddr) (R : Round) (ARP : AddrRoundPair A R) (Sn : Signable) (V : SignableValue Sn) (VBFT : ValueBFT A R V) 
@@ -125,3 +150,4 @@ Module RBACProtocolImpl (A : NetAddr) (R : Round) (ARP : AddrRoundPair A R) (Sn 
 Include RBACProtocol A R ARP Sn V VBFT BTh RBM P TSS0 TSS ACDT CC ACM M RBPk ACPk RBP ACP Pk.
 
 End RBACProtocolImpl.
+*)
